WIP elim stack

new/proof/github_com/goose_lang/goose/testdata/examples/elim_stack.v
@@ -5,17 +5,27 @@ From iris.algebra Require Import auth.
 From New.proof.github_com.goose_lang.goose.model.channel Require Export chan_au_base.
 From New.golang.theory Require Import chan.
 From iris.base_logic.lib Require Import saved_prop.
+From New.proof Require Import strings time sync.
+From New.golang.theory Require Import struct string chan.
 From New.generatedproof.github_com.goose_lang.goose.testdata.examples Require Import channel.
 
+Import chan_spec_raw_examples.
+
+Set Default Proof Using "Type".
+
 Class elimStackGhostStateG Σ := ElimStackGhostStateG {
-  stack_listG :: ghost_varG Σ (list (go_string));
-  push_parked_propG :: savedPropG Σ;
-  pop_parked_predG :: savedPredG Σ (go_string * bool);
+  stack_listG        : ghost_varG Σ (list (go_string));
+  push_parked_propG  : savedPropG Σ;
+  pop_parked_predG   : savedPredG Σ (go_string * bool);
+  elim_chanG         : chanGhostStateG Σ go_string
 }.
 
 Definition elimStackGhostStateΣ : gFunctors :=
-  #[ ghost_varΣ (list (go_string));
-     savedPropΣ; savedPredΣ (go_string * bool) ].
+  #[ ghost_varΣ (list (go_string))
+   ; savedPropΣ
+   ; savedPredΣ (go_string * bool)
+   ; chanGhostStateΣ go_string
+   ].
 
 #[global] Instance subG_elimStackGhostStateG Σ :
   subG elimStackGhostStateΣ Σ → elimStackGhostStateG Σ.
@@ -23,8 +33,15 @@ Proof. solve_inG. Qed.
 
 Section elim_stack.
 Context `{hG: heapGS Σ, !ffi_semantics _ _}.
-Context `{!chanGhostStateG Σ go_string}.
 Context `{!elimStackGhostStateG Σ}.
+Context `{!globalsGS Σ} {go_ctx : GoContext}.
+#[global] Instance : IsPkgInit chan_spec_raw_examples := define_is_pkg_init True%I.
+#[global] Instance : GetIsPkgInitWf chan_spec_raw_examples := build_get_is_pkg_init_wf.
+
+#[local] Existing Instance stack_listG.
+#[local] Existing Instance push_parked_propG.
+#[local] Existing Instance pop_parked_predG.
+#[local] Existing Instance elim_chanG.
 
 Record stack_names := {
   stack_state_name : gname;
@@ -34,10 +51,10 @@ Record stack_names := {
 }.
 
 (** Abstract stack representation *)
-Definition stack_rep (γ: gname) (q: Qp) (l: list (go_string)) : iProp Σ :=
+#[local] Definition stack_rep (γ: gname) (q: Qp) (l: list (go_string)) : iProp Σ :=
   ghost_var γ q l.
 
-Notation stack_rep_full γ l := (stack_rep γ 1 l).
+#[local] Notation stack_rep_full γ l := (stack_rep γ 1 l).
 Notation stack_rep_half γ l := (stack_rep γ (1/2)%Qp l).
 
 Lemma stack_rep_agree γ q1 q2 l1 l2 :
@@ -48,16 +65,12 @@ Qed.
 
 Lemma stack_rep_update γ l l' :
   stack_rep_full γ l ==∗ stack_rep_full γ l'.
-Proof.
-  iApply ghost_var_update.
-Qed.
+Proof. iApply ghost_var_update. Qed.
 
 Lemma stack_rep_halves_update γ l1 l2 l' :
   stack_rep_half γ l1 -∗ stack_rep_half γ l2 ==∗
   stack_rep_half γ l' ∗ stack_rep_half γ l'.
-Proof.
-  iApply ghost_var_update_halves.
-Qed.
+Proof. iApply ghost_var_update_halves. Qed.
 
 (** Atomic updates for push and pop *)
 Definition push_au (s: loc) (v: go_string) (γ: gname) (Φ: iProp Σ) : iProp Σ :=
@@ -77,12 +90,6 @@ Definition pop_au (s: loc) (γ: gname) (Φ: go_string → bool → iProp Σ) : i
 Definition PopK (Φ : go_string → bool → iProp Σ) : (go_string * bool) → iProp Σ :=
   λ '(v,b), Φ v b.
 
-(** Push token: the capability to logically push a value onto the abstract stack *)
-Definition push_token (v: go_string) (γ: gname) : iProp Σ :=
-  |={⊤,∅}=> ∃ l,
-    stack_rep_half γ l ∗
-    (stack_rep_half γ (v :: l) ={∅,⊤}=∗ True).
-
 (** Stack invariant: protected by mutex
     Contains physical stack + push tokens for each element *)
 Definition stack_inv (s: loc) (γ: stack_names) : iProp Σ :=
@@ -90,45 +97,37 @@ Definition stack_inv (s: loc) (γ: stack_names) : iProp Σ :=
     "Hstack" ∷ s ↦s[(chan_spec_raw_examples.EliminationStack) :: "stack"] slice_val ∗
     "Hslice" ∷ own_slice slice_val (DfracOwn 1) physical ∗
     "Hslice_cap" ∷ own_slice_cap (go_string) slice_val (DfracOwn 1) ∗
-    
-    (* For each value in physical stack, we have a push token *)
-    "Htokens" ∷ [∗ list] v ∈ physical, push_token v γ.(stack_state_name).
+    "Hlog2phys" ∷ stack_rep_half γ.(stack_state_name) physical .
 
 (* Exchanger invariant: the state machine for elimination *)
 Definition exchanger_inv (s: loc) (ch: loc) (γ: stack_names) : iProp Σ :=
   ∃ (ch_state: chan_rep.t (go_string)),
     "chan_state" ∷ own_channel ch 0 ch_state γ.(exch_chan_name) ∗
-    
     "logical" ∷ match ch_state with
       | chan_rep.Idle =>
           ∃ (Φpush: iProp Σ) (Φpop: go_string → bool → iProp Σ),
             "push_saved" ∷ saved_prop_own γ.(push_parked_prop_name) (DfracOwn 1) Φpush ∗
             "pop_saved" ∷ saved_pred_own γ.(pop_parked_pred_name) (DfracOwn 1) (PopK Φpop)
-      
       | chan_rep.SndPending v =>
           ∃ (Φpush: iProp Σ) (Φpop: go_string → bool → iProp Σ),
             "push_saved" ∷ saved_prop_own γ.(push_parked_prop_name) (DfracOwn (1/2)) Φpush ∗
             "pop_saved" ∷ saved_pred_own γ.(pop_parked_pred_name) (DfracOwn 1) (PopK Φpop) ∗
             "push_au" ∷ push_au s v γ.(stack_state_name) Φpush
-      
       | chan_rep.RcvPending =>
           ∃ (Φpush: iProp Σ) (Φpop: go_string → bool → iProp Σ),
             "push_saved" ∷ saved_prop_own γ.(push_parked_prop_name) (DfracOwn 1) Φpush ∗
             "pop_saved" ∷ saved_pred_own γ.(pop_parked_pred_name) (DfracOwn (1/2)) (PopK Φpop) ∗
             "pop_au" ∷ pop_au s γ.(stack_state_name) Φpop
-      
       | chan_rep.SndCommit v =>
           ∃ (Φpush: iProp Σ) (Φpop: go_string → bool → iProp Σ),
             "push_saved" ∷ saved_prop_own γ.(push_parked_prop_name) (DfracOwn (1/2)) Φpush ∗
             "pop_saved" ∷ saved_pred_own γ.(pop_parked_pred_name) (DfracOwn (1/2)) (PopK Φpop) ∗
             "pop_complete" ∷ Φpop v true
-      
       | chan_rep.RcvCommit =>
           ∃ (Φpush: iProp Σ) (Φpop: go_string → bool → iProp Σ),
             "push_saved" ∷ saved_prop_own γ.(push_parked_prop_name) (DfracOwn (1/2)) Φpush ∗
             "pop_saved" ∷ saved_pred_own γ.(pop_parked_pred_name) (DfracOwn (1/2)) (PopK Φpop) ∗
             "push_complete" ∷ Φpush
-      
       | _ => False
       end.
 
@@ -149,24 +148,45 @@ Global Instance is_elim_stack_persistent s γ : Persistent (is_elim_stack s γ).
 Proof. apply _. Qed.
 
 Lemma wp_NewEliminationStack :
-  {{{ True }}}
+  {{{ is_pkg_init chan_spec_raw_examples }}}
   @! chan_spec_raw_examples.NewEliminationStack #()
-  {{{ (s: loc) γ, RET #s; 
-      is_elim_stack s γ ∗ stack_rep_full γ.(stack_state_name) []
+  {{{ (s: loc) γ, RET #s;
+      is_elim_stack s γ ∗ stack_rep_half γ.(stack_state_name) []
   }}}.
 Proof.
 Admitted.
 
-Lemma wp_EliminationStack__Push (s: loc) (v: go_string) (γ: stack_names):
+Lemma wp_EliminationStack__Push (s: loc) (v: go_string) (γ: stack_names)  :
   ∀ Φ,
+  s ≠ null ->
   is_elim_stack s γ -∗
+  is_pkg_init chan_spec_raw_examples -∗
   push_au s v γ.(stack_state_name) (Φ #()) -∗
-  WP  chan_spec_raw_examples.EliminationStack__Pushⁱᵐᵖˡ #s #v {{ Φ }}.
+
+  WP chan_spec_raw_examples.EliminationStack__Pushⁱᵐᵖˡ #s #v {{ Φ }}.
 Proof.
+   intros.
+   iIntros "#Hic".
+   iIntros "#Hinit".
+   iIntros "Hau".
+   wp_call.
+  wp_auto_lc 4.
+    iRename select (£1) into "Hlc1".
+
+  wp_apply chan.wp_select_blocking.
+  simpl.
+    iSplit.
+    {
+   wp_apply chan.wp_select_blocking.
+  simpl.
+    iSplit.
+    {
+  wp_start. iIntros "Hau".
 Admitted.
 
-Lemma wp_EliminationStack__Pop (s: loc) (γ: stack_names):
+Lemma wp_EliminationStack__Pop (s: loc) (γ: stack_names) :
   ∀ Φ,
+  is_pkg_init chan_spec_raw_examples -∗
   is_elim_stack s γ -∗
   pop_au s γ.(stack_state_name) (λ v ok, Φ (#v, #ok)%V) -∗
   WP chan_spec_raw_examples.EliminationStack__Popⁱᵐᵖˡ #s {{ Φ }}.
