new/golang/theory/lock_disj.v
@@ -1,0 +1,125 @@
+From New.proof Require Export proof_prelude.
+From New.golang Require Export defn.lock.
+From New.proof Require Export tok_set.
+From New.experiments Require Export glob.
+From Perennial Require Export base.
+
+#[local] Transparent lock.trylock lock.lock lock.unlock.
+
+Section proof.
+Context `{heapGS Σ, !ffi_semantics _ _}.
+Context `{!globalsGS Σ} {go_ctx : GoContext}.
+
+(** This means [m] is a valid mutex with invariant [R] in namespace [N]. *)
+Definition is_lockN (N: namespace) (m: loc) (R : iProp Σ) : iProp Σ :=
+  "#Hinv" ∷ inv N (
+        ∃ b : bool,
+          (m ↦{# 1/4} b) ∗
+          if b then True else m ↦{# 3/4} b ∗ R
+        ) ∗
+  "_" ∷ True.
+#[global] Opaque is_lockN.
+#[local] Transparent is_lockN.
+
+
+(** This resource denotes ownership of the fact that the lock is currently locked. *)
+Definition own_lockN (m: loc) : iProp Σ := m ↦{# 3/4} true.
+#[global] Opaque own_lockN.
+#[local] Transparent own_lockN.
+
+Lemma own_lock_exclusive (m : loc) : own_lockN m -∗ own_lockN m -∗ False.
+Proof.
+  iIntros "H1 H2".
+  iCombine "H1 H2" gives %[Hbad _].
+  exfalso.
+  rewrite go_type_size_unseal in Hbad. naive_solver.
+Qed.
+
+
+Global Instance is_lockN_ne m N : NonExpansive (is_lockN N m).
+Proof. solve_proper. Qed.
+
+Global Instance is_lockN_persistent m N R : Persistent (is_lockN N m R).
+Proof. apply _. Qed.
+
+
+(** Allocate the invariant in an arbitrary namespace [N]. *)
+Theorem init_lockN R E N m :
+  m ↦ false -∗ ▷ R ={E}=∗ is_lockN N m R.
+Proof.
+  iIntros "Hl HR".
+  iEval (rewrite -Qp.quarter_three_quarter) in "Hl".
+iDestruct "Hl" as "[Hl Hr]".  (* now Hl : m ↦{#1/4} false *)
+  iMod (inv_alloc N _ (∃ b:bool, m ↦{#1/4} b ∗ (if b then True else m ↦{#3/4} b ∗ R))
+          with "[Hl HR Hr]") as "#Hinv".
+  { iNext. iExists false. iSplitL "Hl".
+
+    -
+ iExact "Hl".
+    - iFrame. }
+  iModIntro. iFrame "#".
+Qed.
+
+
+Lemma wp_lock_lock N m R :
+  {{{ is_lockN N m R }}}
+    lock.lock #m
+  {{{ RET #(); own_lockN m ∗ R }}}.
+Proof.
+    iLöb as "IH".
+  wp_start as "H". wp_call. iNamed "H".
+  wp_bind (CmpXchg _ _ _).
+  iInv N as ([]) "[Hl HR]".
+  - wp_bind (CmpXchg _ _ _).
+    iApply (wp_typed_cmpxchg_fail (V:=bool) with "[$]").
+    { done. }
+    { naive_solver. }
+    iNext.
+    iIntros "Hl".
+    iModIntro. iSplitL "Hl"; first (iNext; iExists true; eauto).
+    wp_auto.
+    wp_apply "IH"; [iFrame "#" | iFrame].
+  - iDestruct "HR" as "[Hl2 HR]".
+    iCombine "Hl Hl2" as "Hl".
+    rewrite Qp.quarter_three_quarter.
+    wp_bind (CmpXchg _ _ _).
+    iApply (wp_typed_cmpxchg_suc (V:=bool) with "[$]").
+    { constructor. }
+    { done. }
+    iNext. iIntros "Hl".
+    iModIntro.
+    iEval (rewrite -Qp.quarter_three_quarter) in "Hl".
+    iDestruct "Hl" as "[Hl1 Hl2]".
+    iSplitL "Hl1"; first (iNext; iExists true; eauto).
+    rewrite /locked. wp_auto.
+    iApply "HΦ".
+    eauto with iFrame.
+Qed.
+
+
+Lemma wp_lock_unlock N m R :
+  {{{ is_lockN N m R ∗ own_lockN m ∗ ▷ R }}}
+    lock.unlock #m
+  {{{ RET #(); True }}}.
+Proof.
+    wp_start as "(#His & Hlocked & HR)". wp_call.
+  iNamed "His".
+  wp_bind (CmpXchg _ _ _).
+  iInv N as (b) "[>Hl _]".
+
+  unfold own_lockN.
+  iCombine "Hl Hlocked" gives %[_ [=]]. subst.
+  iCombine "Hl Hlocked" as "Hl".
+  rewrite Qp.quarter_three_quarter.
+  iApply (wp_typed_cmpxchg_suc (V:=bool) with "[$]").
+  { econstructor. }
+  { econstructor. }
+  iIntros "!# Hl".
+  iModIntro.
+  iSplitR "HΦ"; last by wp_auto; iApply "HΦ".
+  iEval (rewrite -Qp.quarter_three_quarter) in "Hl".
+  iDestruct "Hl" as "[Hl1 Hl2]".
+  iNext. iExists false. iFrame.
+Qed.
+
+End proof.
